Veritas.Verifier.TSLog.fst
@@ -1,5 +1,7 @@
 module Veritas.Verifier.TSLog
 
+module VG = Veritas.Verifier.Global
+
 let clock_sorted (il: il_vlog{verifiable il}) =
  forall (i j:I.seq_index il). i <= j ==> clock il i `ts_leq` clock il j
 
@@ -72,208 +74,411 @@ let lemma_prefix_verifiable (itsl: its_log) (i:nat{i <= I.length itsl})
     lemma_prefix_clock_sorted itsl i
 
 let create (gl: VG.verifiable_log)
-  =  admit()
-
-let lemma_create_correct (gl: VG.verifiable_log):
-  Lemma (gl = to_g_vlog (create gl)) = admit()
-
-let thread_state (#p:pos) (itsl: its_log p) (tid: valid_tid p): (vs:vtls{Valid? vs}) = 
-  let gl = partition_idx_seq itsl in
-  let tl = VG.thread_log gl tid in
-  VT.verify tl
-
-let lemma_verifier_thread_state_extend (#p:pos) (itsl: its_log p) (i:seq_index itsl):
-  Lemma (thread_state (prefix itsl (i + 1)) (thread_id_of itsl i)== 
-         t_verify_step (thread_state (prefix itsl i) (thread_id_of itsl i))
-                       (vlog_entry_at itsl i)) = 
-  let gl = partition_idx_seq itsl in                       
-  let tid = thread_id_of itsl i in                       
-  
-  admit()                       
-
-(* extended time sequence log (with evict values) 
-let rec time_seq_ext_aux (#p:pos) (itsl: its_log p):
-  Tot (le:vlog_ext{project_seq itsl = to_vlog le})
-  (decreases (length itsl)) =*)
-  (*
-  let m = length itsl in
-  if m = 0 then (
-    lemma_empty itsl;
-    lemma_empty (project_seq itsl);
-    let r = empty #vlog_entry_ext in
-    lemma_empty (to_vlog r);
-    r
-  )
-  else (
-    let (e,id) = telem itsl in
-
-    (* recurse *)
-    let itsl' = its_prefix itsl (m - 1) in
-    let r' = time_seq_ext_aux itsl' in
-
-    (* project seq of itsl and itsl' differ by log entry e *)
-    lemma_project_seq_extend itsl;
-    assert(project_seq itsl = append1 (project_seq itsl') e);
-
-    (* log entries of verifier thread id *)
-    let gl = partition_idx_seq itsl in
-    let l = index gl id in
-    assert(snd (index (g_tid_vlog gl) id) = l);
-
-    (* since l is verifiable, the value at last position is well-defined *)
-    assert(VT.verifiable (id, l));
-    (* prove length l > 0 *)
-    lemma_partition_idx_extend1 itsl;
-
-    if is_evict_to_merkle e then (
-      let v = evict_value (id, l) (length l - 1) in
-      let r = append1 r' (EvictMerkle e v) in
-      lemma_prefix1_append r' (EvictMerkle e v);
-      lemma_map_extend to_vlog_entry r;
-      r
-    )
-    else if is_evict_to_blum e then (
-      let v = evict_value (id, l) (length l - 1) in
-      let r = append1 r' (EvictBlum e v id) in
-      lemma_prefix1_append r' (EvictBlum e v id);
-      lemma_map_extend to_vlog_entry r;
-      r
-    )
-    else (
-      let r = append1 r' (NEvict e) in
-      lemma_prefix1_append r' (NEvict e);
-      lemma_map_extend to_vlog_entry r;
-      r
-    )
-  )
-  *)
-
-
-let rec lemma_its_prefix_ext (#n:pos) (itsl:its_log n) (i:nat{i <= length itsl}):
-  Lemma (requires True)
-        (ensures (time_seq_ext (its_prefix itsl i) = prefix (time_seq_ext itsl) i)) 
-        (decreases (length itsl)) = 
-  let n = length itsl in          
-  if i = n then ()
-  else (
-    assert(n > 0 && i < n);
-
-    if i = n - 1 then
-      admit()
-    else
-
+  = let open VG in
+    assert (forall (tid:seq_index gl). VT.verifiable (thread_log gl tid));
     admit()
-  )
 
+// let lemma_create_correct (gl: VG.verifiable_log):
+//   Lemma (gl = to_g_vlog (create gl)) = admit()
+
+(*thread state after processing ts log - guaranteed to be valid *)
+let thread_state (itsl: its_log) (tid: valid_tid itsl): (vs:vtls{Valid? vs})
+  = admit()
+
+let lemma_verifier_thread_state_extend (itsl: its_log) (i: I.seq_index itsl):
+  Lemma (thread_state_post itsl i == 
+         t_verify_step (thread_state_pre itsl i) (I.index itsl i))
+  = admit()
+
+(* is this an evict add consistent log *)
+let is_eac (itsl: its_log):bool = admit()
+
+let eac_boundary (itsl: neac_log):
+  (i:I.seq_index itsl{is_eac (I.prefix itsl i) &&
+                      not (is_eac (I.prefix itsl (i + 1)))})
+  = admit()
+  
 (* if itsl is eac, then any prefix is also eac *)
-let lemma_eac_implies_prefix_eac (#p:pos) (itsl: eac_ts_log p) (i:nat {i <= length itsl}):
+let lemma_eac_implies_prefix_eac (itsl: eac_log) (i:nat {i <= I.length itsl}):
   Lemma (requires True)
-        (ensures (is_eac_log (its_prefix itsl i)))
-        [SMTPat (its_prefix itsl i)] = admit()
+        (ensures (is_eac (I.prefix itsl i)))
+    = admit()
+  
+(* if the ts log is eac, then its state ops are read-write consistent *)
+let lemma_eac_implies_state_ops_rw_consistent (itsl: eac_log):
+  Lemma (rw_consistent (state_ops itsl))
+  = admit()
+  
+(* the eac state of a key at the end of an its log *)
+let eac_state_of_key (itsl: its_log) (k:key): eac_state 
+  = admit()
 
-(* 
- * when the eac state of a key is Init (no operations on the key yet) no 
- * thread contains the key in its store 
- *)
-let lemma_eac_state_init_store 
-   (#p:pos) 
-   (itsl: eac_ts_log p) (k: key{k <> Root && is_eac_state_init itsl k}) (id:nat{id < p}):
-   Lemma (not (store_contains (thread_store (verifier_thread_state itsl id)) k)) 
-   = admit()
+let lemma_eac_state_of_key_valid (itsl: eac_log) (k:key):
+  Lemma (EACFail <> eac_state_of_key itsl k)
+  = admit()
 
-(* when the eac state of a key is EACEvicted then no thread contains the key in its store *)
-let lemma_eac_state_evicted_store (#p:pos) (itsl: eac_ts_log p) 
-  (k: key{is_eac_state_evicted itsl k}) (id:nat{id < p}):
-    Lemma (not (store_contains (thread_store (verifier_thread_state itsl id)) k)) = admit()
+(* the extended vlog entry to use for eac checking *)
+let vlog_entry_ext_at (itsl: its_log) (i:I.seq_index itsl): 
+  (e:vlog_entry_ext{E.to_vlog_entry e = I.index itsl i})
+  = admit()
+
+(* the eac state transition induced by the i'th entry *)
+let lemma_eac_state_transition (itsl: its_log) (i:I.seq_index itsl):
+  Lemma (eac_state_post itsl i = 
+         eac_add (vlog_entry_ext_at itsl i) (eac_state_pre itsl i))
+  = admit()         
+
+(* if the ith entry does not involve key k, the eac state of k is unchanged *)
+let lemma_eac_state_same (itsl: its_log) (i: I.seq_index itsl) (k: key):
+  Lemma (requires (key_at itsl i <> k))
+        (ensures (eac_state_of_key (I.prefix itsl i) k == 
+                  eac_state_of_key (I.prefix itsl (i + 1)) k))
+  = admit()
+
+let lemma_eac_boundary_state_transition (itsl: neac_log):
+  Lemma (requires True)
+        (ensures (eac_add (vlog_entry_ext_at itsl (eac_boundary itsl))
+                          (eac_boundary_state_pre itsl) = EACFail))
+        [SMTPat (eac_boundary itsl)]
+  = admit()
+
 
 (* when the eac state of a key is "instore" then there is always a previous add *)
-let lemma_eac_state_instore_implies_prev_add (#p:pos) (itsl: eac_ts_log p) (k:key{is_eac_state_instore itsl k}):
-  Lemma (has_some_add_of_key k (project_seq itsl)) = admit()
-
-(* if the eac_state of k is instore, then that k is in the store of the verifier thread of its last add *)
-let lemma_eac_state_instore (#p:pos) (itsl: eac_ts_log p) (k:key{is_eac_state_instore itsl k}):
-  Lemma (store_contains (thread_store (verifier_thread_state itsl (last_add_tid itsl k))) k /\
-         stored_value (thread_store (verifier_thread_state itsl (last_add_tid itsl k))) k = 
-         EACInStore?.v (eac_state_of_key itsl k)) = admit()
-
-let lemma_eac_state_instore_addm (#p:pos) (itsl: eac_ts_log p) (k:key{is_eac_state_instore itsl k}):
-  Lemma (is_add (index (project_seq itsl) (last_add_idx itsl k)) /\
-         store_contains (thread_store (verifier_thread_state itsl (last_add_tid itsl k))) k /\
-         EACInStore?.m (eac_state_of_key itsl k) = 
-         addm_of_entry (index (project_seq itsl) (last_add_idx itsl k)) /\
-         EACInStore?.m (eac_state_of_key itsl k) = 
-         add_method_of (thread_store (verifier_thread_state itsl (last_add_tid itsl k))) k) = admit()
-
-(* if the eac state of k is instore, then k is not in the store of any verifier thread other than 
- * its last add thread *)
-let lemma_eac_state_instore2 (#p:pos) (itsl: eac_ts_log p) 
-  (k:key{is_eac_state_instore itsl k}) (id:nat{id < p}):
-  Lemma (requires (id <> last_add_tid itsl k))
-        (ensures (not (store_contains (thread_store (verifier_thread_state itsl id)) k))) = admit()
-
-let lemma_instore_implies_eac_state_instore (#p:pos) (itsl:eac_ts_log p) (k:key{k <> Root}) (tid:nat{tid < p}):
-  Lemma (store_contains (thread_store (verifier_thread_state itsl tid)) k ==> is_eac_state_instore itsl k) = 
-  admit()
-
-(* the root is always in thread 0 *)
-let lemma_root_in_store0 (#p:pos) (itsl: eac_ts_log p):
-  Lemma (store_contains (thread_store (verifier_thread_state itsl 0)) Root) = admit()
-
-let lemma_root_not_in_store (#p:pos) (itsl: eac_ts_log p) (tid:pos {tid < p}):
-  Lemma (not (store_contains (thread_store (verifier_thread_state itsl tid)) Root)) = admit()
-
+let lemma_eac_state_active_implies_prev_add (itsl: eac_log) 
+  (k:key{is_eac_state_active itsl k}):
+  Lemma (requires True)
+        (ensures (has_some_add_of_key itsl k))
+  //      [SMTPat (is_eac_state_instore itsl k)]
+  = admit()
+  
+(* the converse of the previous, eac state init implies no previous add *)
+let lemma_eac_state_init_no_entry (itsl: eac_log) (k:key):
+  Lemma (requires (is_eac_state_init itsl k))
+        (ensures (not (has_some_entry_of_key itsl k)))
+ = admit()
+ 
+(* add method of an eac state *)
+let lemma_eac_state_addm (itsl: eac_log) (k:key{is_eac_state_instore itsl k}):
+  Lemma (E.add_method_of (eac_state_of_key itsl k) = 
+         V.addm_of_entry (I.index itsl (last_add_idx itsl k)))
+ = admit()
+ 
 (* the evicted value is always of the correct type for the associated key *)
-let lemma_evict_value_correct_type (#p:pos) (itsl: eac_ts_log p) (k:key{is_eac_state_evicted itsl k}):
-  Lemma (is_value_of k (E.value_of (eac_state_of_key itsl k))) = admit()
+let lemma_eac_value_correct_type (itsl: eac_log) (k:key):  
+  Lemma (requires (E.is_eac_state_active (eac_state_of_key itsl k)))
+        (ensures is_value_of k (E.value_of (eac_state_of_key itsl k)))
+ = admit()
+
+
+(* we never see operations on Root so its eac state is always init *)
+let lemma_eac_state_of_root_init (itsl: eac_log):
+  Lemma (is_eac_state_init itsl Root)
+ = admit()
+ 
+(* 
+ * when the eac state of a key is Init (no operations on the key yet) no 
+ * thread contains the key in its store. Valid only for non-root keys 
+ * since we start off with the root in the cache of thread 0
+ *)
+let lemma_eac_state_init_store (itsl: eac_log) (k: key) (tid:valid_tid itsl):
+  Lemma (requires (k <> Root && is_eac_state_init itsl k))
+        (ensures (not (store_contains (thread_store itsl tid) k)))
+ = admit()
+
+
+(* when the eac state of a key is evicted then no thread contains the key in its store *)
+let lemma_eac_state_evicted_store  (itsl: eac_log) (k: key{is_eac_state_evicted itsl k}) 
+  (tid:valid_tid itsl):
+  Lemma (not (store_contains (thread_store itsl tid) k))
+ = admit()
+
+
+(* when the eac_state of k is instore, then k is in the store of a unique verifier thread *)
+let stored_tid (itsl: eac_log) (k:key{is_eac_state_instore itsl k}): 
+  (tid: valid_tid itsl{store_contains (thread_store itsl tid) k})
+ = admit()
+
+
+(* uniqueness: k is not in any store other than stored_tid *)
+let lemma_key_in_unique_store (itsl: eac_log) (k:key) (tid: valid_tid itsl):
+  Lemma (requires (is_eac_state_instore itsl k))
+        (ensures (tid <> stored_tid itsl k ==> not (store_contains (thread_store itsl tid) k)))
+  = admit()         
+
+let lemma_key_in_unique_store2 (itsl: eac_log) (k:key) (tid1 tid2: valid_tid itsl):
+  Lemma (requires (tid1 <> tid2))
+        (ensures (not (store_contains (thread_store itsl tid1) k &&
+                       store_contains (thread_store itsl tid2) k)))
+  = admit()
+
+(* for data keys, the value in the store is the same as the value associated with the eac state *)
+let lemma_eac_stored_value (itsl: eac_log) (k: data_key{is_eac_state_instore itsl k}):
+  Lemma (eac_state_value itsl k = stored_value itsl k)
+  = admit()
+
 
 (* 
- * for keys in a thread store, return the value in the thread store; 
- * for other keys return the last evict value or null (init)
+ * for all keys, the add method stored in the store is the same as the add method associated 
+ * with eac state
  *)
-let eac_value (#n:pos) (itsl: eac_ts_log n) (k:key): value_type_of k = 
-  if k = Root then (
-    lemma_root_in_store0 itsl;
-    stored_value (thread_store (verifier_thread_state itsl 0)) Root
-  )
-  else 
-    let es = eac_state_of_key itsl k in
-    match es with
-    | EACInit -> init_value k 
-    | EACEvictedMerkle v -> lemma_evict_value_correct_type itsl k; v
-    | EACEvictedBlum v _ _ -> lemma_evict_value_correct_type itsl k; v
-    | EACInStore _ _ -> 
-      (* the store where the last add happened contains key k *)
-      let tid = last_add_tid itsl k in
-      let st = thread_store (verifier_thread_state itsl tid) in
-        
-      lemma_eac_state_instore itsl k;
-      assert(store_contains st k);
+let lemma_eac_stored_addm (itsl: eac_log) (k:key{is_eac_state_instore itsl k}):
+  Lemma (E.add_method_of (eac_state_of_key itsl k) = stored_add_method itsl k)
+  = admit()
 
-      stored_value st k
 
-let lemma_eac_value_is_stored_value (#p:pos) (itsl: eac_ts_log p) (k:key) (id:nat{id < p}):
-  Lemma (requires (store_contains (thread_store (verifier_thread_state itsl id)) k))
-        (ensures (eac_value itsl k = 
-                  stored_value (thread_store (verifier_thread_state itsl id)) k)) = admit()
+(* if k is in a verifier store, then its eac_state is instore *)
+let lemma_instore_implies_eac_state_instore (itsl:eac_log) (k:key{k <> Root}) (tid:valid_tid itsl):
+  Lemma (store_contains (thread_store itsl tid) k ==> is_eac_state_instore itsl k)
+  = admit()
+         
+(* the root is always in thread 0 *)
+let lemma_root_in_store0 (itsl: eac_log{thread_count itsl > 0}):
+  Lemma (store_contains (thread_store itsl 0) Root) = admit()
 
-let lemma_eac_value_is_evicted_value (#p:pos) (itsl: eac_ts_log p) (k:key):
+let lemma_root_not_in_store (itsl: eac_log) (tid:valid_tid itsl{tid > 0}):
+  Lemma (not (store_contains (thread_store itsl tid) Root)) = admit()
+  
+(* we use eac constraints to associate a value with each key *)
+let eac_value (itsl: eac_log) (k:key): value_type_of k = admit()
+
+(* eac_value is consistent with stored value *)
+let lemma_eac_value_is_stored_value (itsl: eac_log) (k:key) (tid: valid_tid itsl):  
+  Lemma (requires (store_contains (thread_store itsl tid) k))
+        (ensures (eac_value itsl k = V.stored_value (thread_store itsl tid) k))
+  = admit()        
+
+let lemma_eac_value_is_evicted_value (itsl: eac_log) (k:key):
   Lemma (requires (is_eac_state_evicted itsl k))
-        (ensures (eac_state_evicted_value itsl k = eac_value itsl k)) = admit()
+        (ensures (eac_state_evicted_value itsl k = eac_value itsl k))
+  = admit()        
 
-let lemma_ext_evict_val_is_stored_val (#p:pos) (itsl: its_log p) (i: seq_index itsl):
-  Lemma (requires (is_evict (fst (index itsl i))))
-        (ensures (is_evict_ext (index (time_seq_ext itsl) i) /\
-                  store_contains (thread_store (verifier_thread_state (its_prefix itsl i)
-                                                                      (snd (index itsl i))))
-                                 (V.key_of (fst (index itsl i))) /\
-                  value_ext (index (time_seq_ext itsl) i) = 
-                  stored_value (thread_store (verifier_thread_state (its_prefix itsl i)
-                                                                    (snd (index itsl i))))
-                               (V.key_of (fst (index itsl i))))) = admit()
+let lemma_ext_evict_val_is_stored_val (itsl: its_log) (i: I.seq_index itsl):
+  Lemma (requires (is_evict (I.index itsl i)))
+        (ensures (store_contains (thread_store (I.prefix itsl i) (thread_id_of itsl i)) (key_at itsl i) /\
+                  is_evict_ext (vlog_entry_ext_at itsl i) /\
+                  V.stored_value (thread_store (I.prefix itsl i) (thread_id_of itsl i)) (key_at itsl i) = 
+                  value_ext (vlog_entry_ext_at itsl i)))
+  = admit()        
+
+(* if an evict is not the last entry of a key, then there is a add subsequent to the 
+ * evict *)
+let lemma_evict_has_next_add (itsl: its_log) (i:I.seq_index itsl):
+  Lemma (requires (is_evict (I.index itsl i) /\
+                   exists_sat_elems (is_entry_of_key (key_of (I.index itsl i))) (I.i_seq itsl)) /\
+                   i < last_idx_of_key itsl (key_of (I.index itsl i)))
+        (ensures (has_next_add_of_key itsl i (key_of (I.index itsl i))))
+  = admit()        
+
+let lemma_root_never_evicted (itsl: its_log) (i:I.seq_index itsl):
+  Lemma (requires (is_evict (I.index itsl i)))
+        (ensures (V.key_of (I.index itsl i) <> Root))
+  = admit()        
+
+(* since the itsl is sorted by clock, the following lemma holds *)
+let lemma_clock_ordering (itsl: its_log) (i1 i2: I.seq_index itsl):
+  Lemma (requires (clock itsl i1 `ts_lt` clock itsl i2))
+        (ensures (i1 < i2))
+  = admit()        
+  
+(* the state of each key for an empty log is init *)
+let lemma_init_state_empty (itsl: its_log {I.length itsl = 0}) (k: key):
+  Lemma (eac_state_of_key itsl k = EACInit)
+  = admit()        
+
+(* broken ... but lots of useful stuff below *)
+
+// // let lemma_verifier_thread_state_extend (#p:pos) (itsl: its_log p) (i:seq_index itsl):
+// //   Lemma (thread_state (prefix itsl (i + 1)) (thread_id_of itsl i)== 
+// //          t_verify_step (thread_state (prefix itsl i) (thread_id_of itsl i))
+// //                        (vlog_entry_at itsl i)) = 
+// //   let gl = partition_idx_seq itsl in                       
+// //   let tid = thread_id_of itsl i in                       
+  
+//   admit()                       
+
+// (* extended time sequence log (with evict values) 
+// let rec time_seq_ext_aux (#p:pos) (itsl: its_log p):
+//   Tot (le:vlog_ext{project_seq itsl = to_vlog le})
+//   (decreases (length itsl)) =*)
+//   (*
+//   let m = length itsl in
+//   if m = 0 then (
+//     lemma_empty itsl;
+//     lemma_empty (project_seq itsl);
+//     let r = empty #vlog_entry_ext in
+//     lemma_empty (to_vlog r);
+//     r
+//   )
+//   else (
+//     let (e,id) = telem itsl in
+
+//     (* recurse *)
+//     let itsl' = its_prefix itsl (m - 1) in
+//     let r' = time_seq_ext_aux itsl' in
+
+//     (* project seq of itsl and itsl' differ by log entry e *)
+//     lemma_project_seq_extend itsl;
+//     assert(project_seq itsl = append1 (project_seq itsl') e);
+
+//     (* log entries of verifier thread id *)
+//     let gl = partition_idx_seq itsl in
+//     let l = index gl id in
+//     assert(snd (index (g_tid_vlog gl) id) = l);
+
+//     (* since l is verifiable, the value at last position is well-defined *)
+//     assert(VT.verifiable (id, l));
+//     (* prove length l > 0 *)
+//     lemma_partition_idx_extend1 itsl;
+
+//     if is_evict_to_merkle e then (
+//       let v = evict_value (id, l) (length l - 1) in
+//       let r = append1 r' (EvictMerkle e v) in
+//       lemma_prefix1_append r' (EvictMerkle e v);
+//       lemma_map_extend to_vlog_entry r;
+//       r
+//     )
+//     else if is_evict_to_blum e then (
+//       let v = evict_value (id, l) (length l - 1) in
+//       let r = append1 r' (EvictBlum e v id) in
+//       lemma_prefix1_append r' (EvictBlum e v id);
+//       lemma_map_extend to_vlog_entry r;
+//       r
+//     )
+//     else (
+//       let r = append1 r' (NEvict e) in
+//       lemma_prefix1_append r' (NEvict e);
+//       lemma_map_extend to_vlog_entry r;
+//       r
+//     )
+//   )
+//   *)
 
 
-let lemma_evict_has_next_add (#p:pos) (itsl: its_log p) (i:seq_index itsl):
-  Lemma (requires (is_evict (index itsl i) /\
-                   exists_sat_elems (entry_of_key (key_of (index itsl i))) itsl) /\
-                   i < last_idx_of_key itsl (key_of (index itsl i)))
-        (ensures (has_next_add_of_key itsl i (key_of (index itsl i)))) = admit()
+// let rec lemma_its_prefix_ext (#n:pos) (itsl:its_log n) (i:nat{i <= length itsl}):
+//   Lemma (requires True)
+//         (ensures (time_seq_ext (its_prefix itsl i) = prefix (time_seq_ext itsl) i)) 
+//         (decreases (length itsl)) = 
+//   let n = length itsl in          
+//   if i = n then ()
+//   else (
+//     assert(n > 0 && i < n);
+
+//     if i = n - 1 then
+//       admit()
+//     else
+
+//     admit()
+//   )
+
+// (* if itsl is eac, then any prefix is also eac *)
+// let lemma_eac_implies_prefix_eac (#p:pos) (itsl: eac_ts_log p) (i:nat {i <= length itsl}):
+//   Lemma (requires True)
+//         (ensures (is_eac_log (its_prefix itsl i)))
+//         [SMTPat (its_prefix itsl i)] = admit()
+
+// (* 
+//  * when the eac state of a key is Init (no operations on the key yet) no 
+//  * thread contains the key in its store 
+//  *)
+// let lemma_eac_state_init_store 
+//    (#p:pos) 
+//    (itsl: eac_ts_log p) (k: key{k <> Root && is_eac_state_init itsl k}) (id:nat{id < p}):
+//    Lemma (not (store_contains (thread_store (verifier_thread_state itsl id)) k)) 
+//    = admit()
+
+// (* when the eac state of a key is EACEvicted then no thread contains the key in its store *)
+// let lemma_eac_state_evicted_store (#p:pos) (itsl: eac_ts_log p) 
+//   (k: key{is_eac_state_evicted itsl k}) (id:nat{id < p}):
+//     Lemma (not (store_contains (thread_store (verifier_thread_state itsl id)) k)) = admit()
+
+// (* when the eac state of a key is "instore" then there is always a previous add *)
+// let lemma_eac_state_instore_implies_prev_add (#p:pos) (itsl: eac_ts_log p) (k:key{is_eac_state_instore itsl k}):
+//   Lemma (has_some_add_of_key k (project_seq itsl)) = admit()
+
+// (* if the eac_state of k is instore, then that k is in the store of the verifier thread of its last add *)
+// let lemma_eac_state_instore (#p:pos) (itsl: eac_ts_log p) (k:key{is_eac_state_instore itsl k}):
+//   Lemma (store_contains (thread_store (verifier_thread_state itsl (last_add_tid itsl k))) k /\
+//          stored_value (thread_store (verifier_thread_state itsl (last_add_tid itsl k))) k = 
+//          EACInStore?.v (eac_state_of_key itsl k)) = admit()
+
+// let lemma_eac_state_instore_addm (#p:pos) (itsl: eac_ts_log p) (k:key{is_eac_state_instore itsl k}):
+//   Lemma (is_add (index (project_seq itsl) (last_add_idx itsl k)) /\
+//          store_contains (thread_store (verifier_thread_state itsl (last_add_tid itsl k))) k /\
+//          EACInStore?.m (eac_state_of_key itsl k) = 
+//          addm_of_entry (index (project_seq itsl) (last_add_idx itsl k)) /\
+//          EACInStore?.m (eac_state_of_key itsl k) = 
+//          add_method_of (thread_store (verifier_thread_state itsl (last_add_tid itsl k))) k) = admit()
+
+// (* if the eac state of k is instore, then k is not in the store of any verifier thread other than 
+//  * its last add thread *)
+// let lemma_eac_state_instore2 (#p:pos) (itsl: eac_ts_log p) 
+//   (k:key{is_eac_state_instore itsl k}) (id:nat{id < p}):
+//   Lemma (requires (id <> last_add_tid itsl k))
+//         (ensures (not (store_contains (thread_store (verifier_thread_state itsl id)) k))) = admit()
+
+// let lemma_instore_implies_eac_state_instore (#p:pos) (itsl:eac_ts_log p) (k:key{k <> Root}) (tid:nat{tid < p}):
+//   Lemma (store_contains (thread_store (verifier_thread_state itsl tid)) k ==> is_eac_state_instore itsl k) = 
+//   admit()
+
+// (* the root is always in thread 0 *)
+// let lemma_root_in_store0 (#p:pos) (itsl: eac_ts_log p):
+//   Lemma (store_contains (thread_store (verifier_thread_state itsl 0)) Root) = admit()
+
+// let lemma_root_not_in_store (#p:pos) (itsl: eac_ts_log p) (tid:pos {tid < p}):
+//   Lemma (not (store_contains (thread_store (verifier_thread_state itsl tid)) Root)) = admit()
+
+// (* the evicted value is always of the correct type for the associated key *)
+// let lemma_evict_value_correct_type (#p:pos) (itsl: eac_ts_log p) (k:key{is_eac_state_evicted itsl k}):
+//   Lemma (is_value_of k (E.value_of (eac_state_of_key itsl k))) = admit()
+
+// (* 
+//  * for keys in a thread store, return the value in the thread store; 
+//  * for other keys return the last evict value or null (init)
+//  *)
+// let eac_value (#n:pos) (itsl: eac_ts_log n) (k:key): value_type_of k = 
+//   if k = Root then (
+//     lemma_root_in_store0 itsl;
+//     stored_value (thread_store (verifier_thread_state itsl 0)) Root
+//   )
+//   else 
+//     let es = eac_state_of_key itsl k in
+//     match es with
+//     | EACInit -> init_value k 
+//     | EACEvictedMerkle v -> lemma_evict_value_correct_type itsl k; v
+//     | EACEvictedBlum v _ _ -> lemma_evict_value_correct_type itsl k; v
+//     | EACInStore _ _ -> 
+//       (* the store where the last add happened contains key k *)
+//       let tid = last_add_tid itsl k in
+//       let st = thread_store (verifier_thread_state itsl tid) in
+        
+//       lemma_eac_state_instore itsl k;
+//       assert(store_contains st k);
+
+//       stored_value st k
+
+// let lemma_eac_value_is_stored_value (#p:pos) (itsl: eac_ts_log p) (k:key) (id:nat{id < p}):
+//   Lemma (requires (store_contains (thread_store (verifier_thread_state itsl id)) k))
+//         (ensures (eac_value itsl k = 
+//                   stored_value (thread_store (verifier_thread_state itsl id)) k)) = admit()
+
+// let lemma_eac_value_is_evicted_value (#p:pos) (itsl: eac_ts_log p) (k:key):
+//   Lemma (requires (is_eac_state_evicted itsl k))
+//         (ensures (eac_state_evicted_value itsl k = eac_value itsl k)) = admit()
+
+// let lemma_ext_evict_val_is_stored_val (#p:pos) (itsl: its_log p) (i: seq_index itsl):
+//   Lemma (requires (is_evict (fst (index itsl i))))
+//         (ensures (is_evict_ext (index (time_seq_ext itsl) i) /\
+//                   store_contains (thread_store (verifier_thread_state (its_prefix itsl i)
+//                                                                       (snd (index itsl i))))
+//                                  (V.key_of (fst (index itsl i))) /\
+//                   value_ext (index (time_seq_ext itsl) i) = 
+//                   stored_value (thread_store (verifier_thread_state (its_prefix itsl i)
+//                                                                     (snd (index itsl i))))
+//                                (V.key_of (fst (index itsl i))))) = admit()
+
+
+// let lemma_evict_has_next_add (#p:pos) (itsl: its_log p) (i:seq_index itsl):
+//   Lemma (requires (is_evict (index itsl i) /\
+//                    exists_sat_elems (entry_of_key (key_of (index itsl i))) itsl) /\
+//                    i < last_idx_of_key itsl (key_of (index itsl i)))
+//         (ensures (has_next_add_of_key itsl i (key_of (index itsl i)))) = admit()
