Makefile
@@ -17,13 +17,12 @@ FSTAR_FILES := Veritas.BinTree.fsti Veritas.BinTree.fst \
                Veritas.MultiSet.fsti Veritas.MultiSet.fst \
                Veritas.MultiSetHash.fsti Veritas.MultiSetHash.fst \
                Veritas.Hash.fsti \
-               Veritas.Interleave.fsti \
-               Veritas.Interleave.fst \
+               Veritas.Interleave.fsti Veritas.Interleave.fst \
                Veritas.Verifier.fst \
 	       Veritas.Verifier.Thread.fsti Veritas.Verifier.Thread.fst \
                Veritas.Verifier.Global.fsti Veritas.Verifier.Global.fst \
                Veritas.EAC.fsti Veritas.EAC.fst \
-               Veritas.Verifier.TSLog.fsti  \
+               Veritas.Verifier.TSLog.fsti Veritas.Verifier.TSLog.fst \
 	       Veritas.Verifier.Blum.fsti Veritas.Verifier.Blum.fst \
                Veritas.Verifier.Merkle.fsti  \
                Veritas.Verifier.EAC.fst \
